correctness/RegexCorrectness/Backtracker/Traversal/Lemmas.lean
@@ -10,23 +10,23 @@ namespace Regex.Backtracker
 namespace captureNextAux
 
 variable {nfa : NFA} {wf : nfa.WellFormed} {startIdx maxIdx : Nat} {bit₀ bit : BoundedIterator startIdx maxIdx}
-  {visited₀ visited : BitMatrix nfa.nodes.size (maxIdx + 1 - startIdx)} {stack : List (StackEntry HistoryStrategy nfa startIdx maxIdx)}
-
-theorem PathClosure.preserves {result} (hres : captureNextAux HistoryStrategy nfa wf startIdx maxIdx visited [⟨HistoryStrategy.empty, ⟨nfa.start, wf.start_lt⟩, bit⟩] = result)
-  (isNone : result.1 = .none) (v : bit.Valid) (isNextN : bit.IsNextNOf bit₀) (cls : PathClosure bit₀ visited) :
-  PathClosure bit₀ result.2 := by
-  have cinv : ClosureInv bit₀ visited [⟨HistoryStrategy.empty, ⟨nfa.start, wf.start_lt⟩, bit⟩] := by
-    intro state bit state' bit' update isNextN hmem step
-    exact .inl (cls state bit state' bit' (List.ofOption update) isNextN hmem (.last step))
-  exact path_closure hres isNone isNextN cinv (StackInv.intro v)
+  {visited : BitMatrix nfa.nodes.size (maxIdx + 1 - startIdx)} {stack : List (StackEntry HistoryStrategy nfa startIdx maxIdx)}
 
 theorem mem_or_path_of_mem_of_none {result} (hres : captureNextAux HistoryStrategy nfa wf startIdx maxIdx visited [⟨HistoryStrategy.empty, ⟨nfa.start, wf.start_lt⟩, bit⟩] = result)
   (isNone : result.1 = .none) (v : bit.Valid) :
   VisitedInv wf bit visited result.2 :=
   visited_inv_of_none hres isNone VisitedInv.rfl (StackInv.intro v)
 
+theorem PathClosure.preserves {result} (hres : captureNextAux HistoryStrategy nfa wf startIdx maxIdx visited [⟨HistoryStrategy.empty, ⟨nfa.start, wf.start_lt⟩, bit⟩] = result)
+  (isNone : result.1 = .none) (reaches₀ : bit₀.Reaches bit) (cls : PathClosure bit₀ visited) :
+  PathClosure bit₀ result.2 := by
+  have cinv : ClosureInv bit₀ visited [⟨HistoryStrategy.empty, ⟨nfa.start, wf.start_lt⟩, bit⟩] := by
+    intro state bit state' bit' update reaches hmem step
+    exact .inl (cls state bit state' bit' (List.ofOption update) reaches hmem (.last step))
+  exact path_closure hres isNone reaches₀ cinv (StackInv.intro reaches₀.validR)
+
 theorem mem_of_path_of_none {result} (hres : captureNextAux HistoryStrategy nfa wf startIdx maxIdx visited [⟨HistoryStrategy.empty, ⟨nfa.start, wf.start_lt⟩, bit⟩] = result)
-  (isNone : result.1 = .none) (v : bit.Valid) (isNextN : bit.IsNextNOf bit₀) (cls : PathClosure bit₀ visited)
+  (isNone : result.1 = .none) (reaches₀ : bit₀.Reaches bit) (cls : PathClosure bit₀ visited)
   (bit' : BoundedIterator startIdx maxIdx) (state : Fin nfa.nodes.size) (update : List (Nat × Pos)) (path : Path nfa wf bit.it bit'.it state update) :
   result.2.get state bit'.index := by
   have mem_start : result.2.get ⟨nfa.start, wf.start_lt⟩ bit.index := hres ▸ mem_stack_top ⟨HistoryStrategy.empty, ⟨nfa.start, wf.start_lt⟩, bit⟩ [] rfl
@@ -35,28 +35,28 @@ theorem mem_of_path_of_none {result} (hres : captureNextAux HistoryStrategy nfa 
     have eq : bit' = bit := BoundedIterator.ext eqit
     simpa [eq, ←eqstate] using mem_start
   | .inr path =>
-    have cls' : PathClosure bit₀ result.2 := cls.preserves hres isNone v isNextN
-    exact cls' ⟨nfa.start, wf.start_lt⟩ bit state bit' update isNextN mem_start path
+    have cls' : PathClosure bit₀ result.2 := cls.preserves hres isNone reaches₀
+    exact cls' ⟨nfa.start, wf.start_lt⟩ bit state bit' update reaches₀ mem_start path
 
 theorem mem_iff_mem_or_path_of_none {result} (hres : captureNextAux HistoryStrategy nfa wf startIdx maxIdx visited [⟨HistoryStrategy.empty, ⟨nfa.start, wf.start_lt⟩, bit⟩] = result)
-  (isNone : result.1 = .none) (v : bit.Valid) (isNextN : bit.IsNextNOf bit₀) (cls : PathClosure bit₀ visited)
-  (bit' : BoundedIterator startIdx maxIdx) (state : Fin nfa.nodes.size) (isNextN' : bit'.IsNextNOf bit) :
+  (isNone : result.1 = .none) (reaches₀ : bit₀.Reaches bit) (cls : PathClosure bit₀ visited)
+  (bit' : BoundedIterator startIdx maxIdx) (state : Fin nfa.nodes.size) (reaches : bit.Reaches bit') :
   result.2.get state bit'.index ↔ visited.get state bit'.index ∨ ∃ update, Path nfa wf bit.it bit'.it state update := by
   apply Iff.intro
   . intro mem
-    exact mem_or_path_of_mem_of_none hres isNone v state bit' isNextN' mem
+    exact mem_or_path_of_mem_of_none hres isNone reaches₀.validR state bit' reaches mem
   . intro h
     match h with
     | .inl mem => exact hres ▸ mem_of_mem_visited mem
-    | .inr ⟨update, path⟩ => exact mem_of_path_of_none hres isNone v isNextN cls bit' state update path
+    | .inr ⟨update, path⟩ => exact mem_of_path_of_none hres isNone reaches₀ cls bit' state update path
 
 end captureNextAux
 
 namespace captureNext.go
 
-open captureNextAux (StackInv VisitedInv NotDoneInv)
+open captureNextAux (StackInv NotDoneInv PathClosure)
 
-variable {nfa : NFA} {wf : nfa.WellFormed} {startIdx maxIdx : Nat} {bit₀ bit : BoundedIterator startIdx maxIdx} {visited₀ visited : BitMatrix nfa.nodes.size (maxIdx + 1 - startIdx)}
+variable {nfa : NFA} {wf : nfa.WellFormed} {startIdx maxIdx : Nat} {bit₀ bit : BoundedIterator startIdx maxIdx} {visited : BitMatrix nfa.nodes.size (maxIdx + 1 - startIdx)}
 
 theorem not_done_of_none {result} (hres : go HistoryStrategy nfa wf startIdx maxIdx bit visited = result)
   (isNone : result.1 = .none)
@@ -74,6 +74,51 @@ theorem not_done_of_none {result} (hres : go HistoryStrategy nfa wf startIdx max
     rw [captureNext.go_not_found_end haux hnext] at hres
     have ndinv' : NotDoneInv visited' := captureNextAux.not_done_of_none haux rfl ndinv
     simpa [←hres] using ndinv'
+
+structure Inv (wf : nfa.WellFormed) (bit₀ bit : BoundedIterator startIdx maxIdx) (visited : BitMatrix nfa.nodes.size (maxIdx + 1 - startIdx)) : Prop where
+  closure : PathClosure bit₀ visited
+  mem_iff_path : ∀ (state' : Fin nfa.nodes.size) (bit' : BoundedIterator startIdx maxIdx),
+    bit₀.Reaches bit' →
+    (visited.get state' bit'.index ↔ ∃ (bitPrev : BoundedIterator startIdx maxIdx) (update : List (Nat × Pos)), bitPrev.BetweenE bit₀ bit ∧ Path nfa wf bitPrev.it bit'.it state' update)
+
+namespace Inv
+
+theorem preservesAux {result} (haux : captureNextAux HistoryStrategy nfa wf startIdx maxIdx visited [⟨HistoryStrategy.empty, ⟨nfa.start, wf.start_lt⟩, bit⟩] = result)
+  (isNone : result.1 = .none) (hnext : bit.hasNext) (reaches : bit₀.Reaches bit)
+  (inv : Inv wf bit₀ bit visited) :
+  Inv wf bit₀ (bit.next hnext) result.2 := by
+  refine ⟨inv.closure.preserves haux isNone reaches, ?_⟩
+  intro state' bit' reaches'
+  rw [captureNextAux.mem_iff_mem_or_path_of_none haux isNone reaches inv.closure bit' state' sorry]
+  rw [inv.mem_iff_path state' bit' reaches']
+  simp only [exists_and_left, BoundedIterator.BetweenE.next_iff reaches.validR hnext, or_and_right,
+    exists_or, existsAndEq, reaches, and_self, true_and]
+
+end Inv
+
+def MemIffPathI (wf : nfa.WellFormed) (bit₀ : BoundedIterator startIdx maxIdx) (visited : BitMatrix nfa.nodes.size (maxIdx + 1 - startIdx)) : Prop :=
+  ∀ (state' : Fin nfa.nodes.size) (bit' : BoundedIterator startIdx maxIdx),
+    bit₀.Reaches bit' →
+    (visited.get state' bit'.index ↔ ∃ (bitPrev : BoundedIterator startIdx maxIdx) (update : List (Nat × Pos)), bitPrev.BetweenE bit₀ bit' ∧ Path nfa wf bitPrev.it bit'.it state' update)
+
+theorem mem_iff_path_of_none {result} (hres : go HistoryStrategy nfa wf startIdx maxIdx bit visited = result)
+  (isNone : result.1 = .none) (inv : Inv wf bit₀ bit visited) :
+  MemIffPathI wf bit₀ result.2 := by
+  induction bit, visited using captureNext.go.induct' HistoryStrategy nfa wf startIdx maxIdx with
+  | found bit visited update visited' haux =>
+    rw [captureNext.go_found haux] at hres
+    simp [←hres] at isNone
+  | not_found_next bit visited visited' haux hnext ih =>
+    rw [captureNext.go_not_found_next haux hnext] at hres
+    exact ih hres (inv.preservesAux haux rfl hnext sorry)
+  | not_found_end bit visited visited' haux hnext =>
+    rw [captureNext.go_not_found_end haux hnext] at hres
+    have eq : bit = bit₀.last := sorry
+    subst bit
+
+    intro state' bit' reaches'
+    have := captureNextAux.mem_iff_mem_or_path_of_none haux rfl sorry inv.closure bit' state' -- ???
+    sorry
 
 end captureNext.go
 
