correctness/RegexCorrectness/Data/BoundedIterator.lean
@@ -30,6 +30,8 @@ theorem byteIdx_lt_next_byteIdx {bit : BoundedIterator startIdx maxIdx} (h : bit
   simp [next, pos, Iterator.next'_eq_next]
   exact String.Iterator.lt_next bit.it
 
+theorem pos_lt_next_pos {bit : BoundedIterator startIdx maxIdx} (h : bit.hasNext) : bit.pos < (bit.next h).pos := byteIdx_lt_next_byteIdx h
+
 theorem valid_of_it_valid {bit : BoundedIterator startIdx maxIdx} (v : bit.it.Valid) : bit.Valid := v.isValid
 
 theorem valid_of_valid {bit : BoundedIterator startIdx maxIdx} (v : bit.Valid) : bit.it.Valid := Iterator.Valid.of_isValid v
@@ -113,42 +115,6 @@ theorem nextn_add (bit : BoundedIterator startIdx maxIdx) (n₁ n₂ : Nat) : bi
     else
       simp [nextn, this, hnext, nextn_not_hasNext hnext]
 
-namespace IsNextNOf
-
-@[simp]
-theorem rfl {bit : BoundedIterator startIdx maxIdx} : bit.IsNextNOf bit := ⟨0, by simp [nextn]⟩
-
-theorem toString {bit bit₀ : BoundedIterator startIdx maxIdx} (h : bit.IsNextNOf bit₀) : bit.toString = bit₀.toString := by
-  have ⟨n, eq⟩ := h
-  simp [eq, nextn_toString]
-
-theorem hasNext_of_hasNext {bit bit₀ : BoundedIterator startIdx maxIdx} (h : bit.IsNextNOf bit₀) (hnext : bit.hasNext) : bit₀.hasNext := by
-  have ⟨n, eq⟩ := h
-  cases n with
-  | zero => simpa [eq] using hnext
-  | succ n =>
-    if hnext₀ : bit₀.hasNext then
-      exact hnext₀
-    else
-      simp [nextn, hnext₀] at eq
-      simpa [eq] using hnext
-
-theorem next {bit bit₀ : BoundedIterator startIdx maxIdx} (h : bit.IsNextNOf bit₀) (hnext : bit.hasNext) : (bit.next hnext).IsNextNOf bit₀ := by
-  have ⟨n, eq⟩ := h
-  exact ⟨n + 1, by simp [eq, nextn_next]⟩
-
-theorem valid {bit bit₀ : BoundedIterator startIdx maxIdx} (h : bit.IsNextNOf bit₀) (v₀ : bit₀.Valid) : bit.Valid := by
-  have ⟨n, eq⟩ := h
-  rw [eq]
-  exact nextn_valid v₀
-
-theorem trans {bit₀ bit₁ bit₂ : BoundedIterator startIdx maxIdx} (h₀ : bit₁.IsNextNOf bit₀) (h₁ : bit₂.IsNextNOf bit₁) : bit₂.IsNextNOf bit₀ := by
-  have ⟨n₀, eq₀⟩ := h₀
-  have ⟨n₁, eq₁⟩ := h₁
-  exact ⟨n₀ + n₁, by simp [eq₀, eq₁, nextn_add]⟩
-
-end IsNextNOf
-
 def ValidFor (l r : List Char) (bit : BoundedIterator startIdx maxIdx) : Prop := bit.it.ValidFor l r
 
 namespace ValidFor
@@ -161,13 +127,27 @@ theorem next {l c r} {bit : BoundedIterator startIdx maxIdx} (vf : ValidFor l (c
   unfold ValidFor at vf
   exact vf.next
 
-theorem next' {l r} {bit : BoundedIterator startIdx maxIdx} (h : bit.hasNext) (vf : ValidFor l r bit) : ∃ c r', ValidFor (c :: l) r' (bit.next h) := by
+theorem next' {l r} {bit : BoundedIterator startIdx maxIdx} (h : bit.hasNext) (vf : ValidFor l r bit) : ∃ c r', r = c :: r' ∧ ValidFor (c :: l) r' (bit.next h) := by
   match r with
   | [] => simp [vf.hasNext] at h
-  | c :: r' => exact ⟨c, r', vf.next⟩
+  | c :: r' => exact ⟨c, r', rfl, vf.next⟩
 
 theorem curr {l c r} {bit : BoundedIterator startIdx maxIdx} (vf : ValidFor l (c :: r) bit) : bit.curr (by simp [vf.hasNext]) = c := by
   simp [BoundedIterator.curr, bit.it.curr'_eq_curr, String.Iterator.ValidFor.curr vf]
+
+theorem toString {l r} {bit : BoundedIterator startIdx maxIdx} (vf : ValidFor l r bit) : bit.toString = ⟨l.reverse ++ r⟩ := by
+  simp [ValidFor] at vf
+  simpa [toString] using vf.toString
+
+theorem valid {l r} {bit : BoundedIterator startIdx maxIdx} (vf : ValidFor l r bit) : bit.Valid := by
+  simp [ValidFor] at vf
+  exact valid_of_it_valid vf.valid
+
+theorem eq {l l' r r'} {bit : BoundedIterator startIdx maxIdx} (vf : ValidFor l r bit) (vf' : ValidFor l' r' bit) : l = l' ∧ r = r' :=
+  Iterator.ValidFor.eq vf vf'
+
+theorem eq_it {l r} {bit bit' : BoundedIterator startIdx maxIdx} (vf : ValidFor l r bit) (vf' : ValidFor l r bit') : bit = bit' :=
+  BoundedIterator.ext (Iterator.ValidFor.eq_it vf vf')
 
 end ValidFor
 
@@ -183,6 +163,136 @@ theorem validFor_of_hasNext {bit : BoundedIterator startIdx maxIdx} (h : bit.has
   | [] => simp [vf.hasNext] at h
   | c :: r' => exact ⟨l, r', by simpa [vf.curr] using vf⟩
 
+theorem next {bit : BoundedIterator startIdx maxIdx} (hnext : bit.hasNext) (v : bit.Valid) : (bit.next hnext).Valid := by
+have ⟨l, r, vf⟩ := v.validFor_of_hasNext hnext
+exact vf.next.valid
+
 end Valid
+
+theorem eq_of_valid_of_next_eq {bit bit' : BoundedIterator startIdx maxIdx} (v : bit.Valid) (v' : bit'.Valid) (hnext : bit.hasNext) (hnext' : bit'.hasNext) (eq : bit.next hnext = bit'.next hnext') : bit = bit' := by
+  have ⟨l, r, vf⟩ := v.validFor_of_hasNext hnext
+  have vfn := vf.next
+  have ⟨l', r', vf'⟩ := v'.validFor_of_hasNext hnext'
+  have vfn' := vf'.next
+
+  have eqs : bit.curr hnext :: l = bit'.curr hnext' :: l' ∧ r = r' := vfn.eq (eq ▸ vfn')
+  simp at eqs
+  simp [eqs] at vf
+
+  exact vf.eq_it vf'
+
+inductive Reaches (bit : BoundedIterator startIdx maxIdx) : BoundedIterator startIdx maxIdx → Prop
+| refl (v : bit.Valid) : Reaches bit bit
+| next {bit' : BoundedIterator startIdx maxIdx} (h : bit.Reaches bit') (hnext : bit'.hasNext) : Reaches bit (bit'.next hnext)
+
+namespace Reaches
+
+theorem trans {bit₁ bit₂ bit₃ : BoundedIterator startIdx maxIdx} (h₁ : Reaches bit₁ bit₂) (h₂ : Reaches bit₂ bit₃) : Reaches bit₁ bit₃ := by
+  induction h₂ with
+  | refl => exact h₁
+  | @next bit' _ hnext ih => exact ih.next hnext
+
+theorem validL {bit₁ bit₂ : BoundedIterator startIdx maxIdx} (h : Reaches bit₁ bit₂) : bit₁.Valid := by
+  induction h with
+  | refl v => exact v
+  | next _ _ ih => exact ih
+
+theorem validR {bit₁ bit₂ : BoundedIterator startIdx maxIdx} (h : Reaches bit₁ bit₂) : bit₂.Valid := by
+  induction h with
+  | refl v => exact v
+  | next _ hnext ih => exact ih.next hnext
+
+theorem toString {bit₁ bit₂ : BoundedIterator startIdx maxIdx} (h : Reaches bit₁ bit₂) : bit₂.toString = bit₁.toString := by
+  induction h with
+  | refl => rfl
+  | next _ _ ih => simp [next_toString, ih]
+
+theorem le_pos {bit₁ bit₂ : BoundedIterator startIdx maxIdx} (h : Reaches bit₁ bit₂) : bit₁.pos ≤ bit₂.pos := by
+  induction h with
+  | refl v => exact Nat.le_refl _
+  | next _ hnext ih => exact Nat.le_of_lt (Nat.lt_of_le_of_lt ih (byteIdx_lt_next_byteIdx hnext))
+
+theorem next_iff' {bit₁ bit₂ bit₂' : BoundedIterator startIdx maxIdx} (v : bit₂.Valid) (hnext : bit₂.hasNext) (eq : bit₂' = bit₂.next hnext) : bit₁.Reaches bit₂' ↔ bit₁.Reaches bit₂ ∨ (bit₁.Valid ∧ bit₁ = bit₂') := by
+  apply Iff.intro
+  . intro h
+    cases h with
+    | refl v => exact .inr ⟨v, rfl⟩
+    | @next bit₂' h hnext' =>
+      have eq : bit₂' = bit₂ := eq_of_valid_of_next_eq h.validR v hnext' hnext eq
+      exact .inl (eq ▸ h)
+  . intro h
+    match h with
+    | .inl h => exact eq ▸ h.next hnext
+    | .inr ⟨v, eq'⟩ => exact eq' ▸ .refl v
+
+@[simp]
+theorem next_iff {bit₁ bit₂ : BoundedIterator startIdx maxIdx} (v : bit₂.Valid) (hnext : bit₂.hasNext) : bit₁.Reaches (bit₂.next hnext) ↔ bit₁.Reaches bit₂ ∨ (bit₁.Valid ∧ bit₁ = bit₂.next hnext) :=
+  next_iff' v hnext rfl
+
+end Reaches
+
+def BetweenI (bit bs be : BoundedIterator startIdx maxIdx) : Prop := bs.Reaches bit ∧ bit.Reaches be
+
+def BetweenE (bit bs be : BoundedIterator startIdx maxIdx) : Prop := bit.pos < be.pos ∧ bit.BetweenI bs be
+
+namespace BetweenI
+
+variable {bit bs be : BoundedIterator startIdx maxIdx}
+
+theorem reachesSE (h : bit.BetweenI bs be) : bs.Reaches be := h.1.trans h.2
+
+theorem le_pos (h : bit.BetweenI bs be) : bit.pos ≤ be.pos := h.2.le_pos
+
+@[simp]
+theorem next_iff (v : be.Valid) (hnext : be.hasNext) : bit.BetweenI bs (be.next hnext) ↔ bit.BetweenI bs be ∨ (bs.Reaches bit ∧ bit = be.next hnext) := by
+  simp [BetweenI, v, hnext, ←and_or_left]
+  intro h
+  simp [h.validR]
+
+theorem iffE : bit.BetweenI bs be ↔ bit.BetweenE bs be ∨ (bs.Reaches bit ∧ bit = be) := by
+  apply Iff.intro
+  . intro h
+    if lt : bit.pos < be.pos then
+      exact .inl ⟨lt, h⟩
+    else
+      have eq_pos : bit.pos = be.pos := by
+        simp [String.Pos.ext_iff]
+        exact Nat.le_antisymm (le_pos h) (Nat.le_of_not_lt lt)
+      have eq : bit = be := by
+        simp [BoundedIterator.ext_pos_iff, eq_pos, h.2.toString]
+      exact .inr ⟨h.1, eq⟩
+  . intro h
+    match h with
+    | .inl ⟨lt, h⟩ => exact h
+    | .inr ⟨h, eq⟩ => exact ⟨h, eq ▸ .refl h.validR⟩
+
+end BetweenI
+
+namespace BetweenE
+
+variable {bit bs be : BoundedIterator startIdx maxIdx}
+
+theorem validE (h : bit.BetweenE bs be) : be.Valid := h.2.2.validR
+
+theorem ne_end (h : bit.BetweenE bs be) : bit ≠ be := by
+  intro eq
+  have lt : bit.pos < be.pos := h.1
+  simp only [eq, String.pos_lt_eq, Nat.lt_irrefl] at lt
+
+theorem next_iffI (v : be.Valid) (hnext : be.hasNext) : bit.BetweenE bs (be.next hnext) ↔ bit.BetweenI bs be := by
+  simp [BetweenE, v, hnext, -String.pos_lt_eq]
+  apply Iff.intro
+  . intro ⟨lt, h⟩
+    match h with
+    | .inl h => exact h
+    | .inr ⟨_, eq⟩ => simp only [eq, String.pos_lt_eq, Nat.lt_irrefl] at lt
+  . intro h
+    exact ⟨Nat.lt_of_le_of_lt (h.le_pos) (pos_lt_next_pos hnext), .inl h⟩
+
+@[simp]
+theorem next_iff (v : be.Valid) (hnext : be.hasNext) : bit.BetweenE bs (be.next hnext) ↔ bit.BetweenE bs be ∨ (bs.Reaches bit ∧ bit = be) := by
+  simp [next_iffI v hnext, BetweenI.iffE]
+
+end BetweenE
 
 end Regex.Data.BoundedIterator
